theories/Compositional_Structures/Basic_Modules/Component_Types/Electoral_Module_Ref.thy
@@ -9,12 +9,12 @@ begin
 type_synonym 'a Electoral_Module_Ref = "'a set \<Rightarrow> 'a Profile_List \<Rightarrow> 'a Result nres"
 
 abbreviation elec_mod_rel_orig :: "('a \<times> 'a) set \<Rightarrow> 
-  (('a set \<Rightarrow> 'a Profile \<Rightarrow> 'a Result) \<times> ('a set \<Rightarrow> 'a Profile \<Rightarrow> 'a Result)) set" where
+  ('a Electoral_Module \<times> 'a Electoral_Module) set" where
   "elec_mod_rel_orig R \<equiv> \<langle>\<langle>R\<rangle>set_rel , \<langle>\<langle>\<langle>R \<times>\<^sub>r R\<rangle>set_rel\<rangle>list_rel , 
   \<langle>R\<rangle>set_rel \<times>\<^sub>r \<langle>R\<rangle>set_rel \<times>\<^sub>r \<langle>R\<rangle>set_rel\<rangle>fun_rel\<rangle>fun_rel" 
 
 abbreviation elec_mod_rel_orig_nres :: "('a \<times> 'a) set \<Rightarrow> 
-  (('a set \<Rightarrow> 'a Profile \<Rightarrow> 'a Result nres) \<times> ('a set \<Rightarrow> 'a Profile \<Rightarrow> 'a Result nres)) set" where
+  (('a set \<Rightarrow> 'a Profile \<Rightarrow> 'a Result nres) \<times> ('a::{default, linorder, heap, hashable} set \<Rightarrow> 'a Profile \<Rightarrow> 'a Result nres)) set" where
   "elec_mod_rel_orig_nres R \<equiv> \<langle>\<langle>R\<rangle>set_rel , \<langle>\<langle>\<langle>R \<times>\<^sub>r R\<rangle>set_rel\<rangle>list_rel , 
   \<langle>\<langle>R\<rangle>set_rel \<times>\<^sub>r \<langle>R\<rangle>set_rel \<times>\<^sub>r \<langle>R\<rangle>set_rel\<rangle>nres_rel\<rangle>fun_rel\<rangle>fun_rel" 
 
