theories/Borda_Rule_Ref.thy
@@ -5,7 +5,15 @@ theory Borda_Rule_Ref
 begin
 
 definition borda_rule_sep where
-  "borda_rule_sep A p \<equiv> elector_sep borda_elim_sepref (A, p)"
+  "borda_rule_sep A p \<equiv> elector_sep borda_elim_sep (A, p)"
 
+interpretation borda_rule_impl: elector_ref borda_ref borda_elim_sep borda
+  apply unfold_locales
+  subgoal using borda_elim_sep.refine .
+  subgoal using borda_sound .
+  subgoal apply (intro frefI) using borda_ref_correct[THEN frefD] by auto
+  done
+
+lemmas borda_rule_correct = borda_rule_impl.elector_sep_correct
 
 end
